src/ILTacLtac.v
@@ -21,10 +21,11 @@ Module SEP_REIFY := ReifySepExpr.ReifySepExpr ST SEP.
 (** Cancellation **)
 (******************)
 (** The parameters are the following.
+ ** - [bf] [bb] the forward and backward unfolding bounds
  ** - [isConst] is an ltac [* -> bool]
  ** - [ext] is a [TypedPackage .. .. .. .. ..]
  **)
-Ltac sep_canceler isConst ext :=
+Ltac sep_canceler bf bb isConst ext :=
   try change_to_himp;
   (let ext' :=
     (match ext with
@@ -103,7 +104,7 @@ Ltac sep_canceler isConst ext :=
                             Peano_dec.eq_nat_dec nat_rec nat_rect eq_rec_r eq_rect eq_rec 
                             f_equal eq_sym ]; exact proofs ) ; 
                       change (SEP.himp funcsV predsV uvars nil L R) ;
-                      apply (@CancelTacIL.ApplyCancelSep_slice typesV funcsV predsV 
+                      apply (@CancelTacIL.ApplyCancelSep_slice bf bb typesV funcsV predsV 
                         (TacPackIL.ILAlgoTypes.Algos ext typesV)
                         (@TacPackIL.ILAlgoTypes.Algos_correct ext typesV funcsV predsV)
                         uvars L R puresV puresPfV); 
@@ -123,13 +124,11 @@ Ltac sep_canceler isConst ext :=
 (** Symbolic Execution **)
 (************************)
 (** NOTE:
+ ** - [bf] the forward unfolding bound
  ** - [isConst] is an ltac function of type [* -> bool]
  ** - [ext] is the extension. it is a value of type [TypedPackage]
- ** - [simplifier] is an ltac that takes a hypothesis names and simplifies it
- **     (this should be implmented using [cbv beta iota zeta delta [ ... ] in H])
- **     (it is recommended/necessary to call [sym_evaluator] or import its simplification)
  **)
-Ltac sym_eval isConst ext :=
+Ltac sym_eval bf isConst ext :=
 (*TIME  start_timer "sym_eval:init" ; *)
   let rec init_from st :=
     match goal with
@@ -279,7 +278,7 @@ Ltac sym_eval isConst ext :=
                            let g := eval cbv delta [ new ] in new in
                            let result := fresh in
                            assert (result : g) by 
-                             (generalize (@SymILTac.ApplySymEval_slice_no_heap typesV funcsV predsV
+                             (generalize (@SymILTac.ApplySymEval_slice_no_heap bf typesV funcsV predsV
                                  (@TacPackIL.ILAlgoTypes.Algos ext typesV)
                                  (@TacPackIL.ILAlgoTypes.Algos_correct ext typesV funcsV predsV)
                                  stn uvarsV fin_state st isV isD cs sp_v rv_v rp_v puresV
@@ -320,7 +319,7 @@ Ltac sym_eval isConst ext :=
                              let g := eval cbv delta [ new ] in new in
                              let result := fresh in
                              assert (result : g) by  
-                               (generalize (@SymILTac.ApplySymEval_slice_heap typesV funcsV predsV
+                               (generalize (@SymILTac.ApplySymEval_slice_heap bb typesV funcsV predsV
                                  (@TacPackIL.ILAlgoTypes.Algos ext typesV)
                                  (@TacPackIL.ILAlgoTypes.Algos_correct ext typesV funcsV predsV)
                                  stn uvarsV fin_state st isV isD cs sp_v rv_v rp_v puresV SF
@@ -339,214 +338,3 @@ Ltac sym_eval isConst ext :=
           end
       end
   end.
-
-(*
-Ltac sym_eval isConst ext simplifier :=
-(*TIME  start_timer "sym_eval:init" ; *)
-  let rec init_from st :=
-    match goal with
-      | [ H : evalInstrs _ ?st' _ = Some st |- _ ] => init_from st'
-      | [ |- _ ] => st
-    end
-  in          
-  let stn_st_SF :=
-    match goal with
-      | [ H : PropX.interp _ (![ ?SF ] ?X) |- _ ] => 
-        let SF := eval unfold empB, injB, injBX, starB, exB, hvarB in SF in
-        constr:((X, (SF, H)))
-      | [ H : Structured.evalCond _ _ _ ?stn ?st = _ |- _ ] => 
-        let st := init_from st in
-        constr:(((stn, st), tt))
-      | [ H : IL.evalInstrs ?stn ?st _ = _ |- _ ] =>
-        let st := init_from st in
-        constr:(((stn, st), tt))
-      | [ |- _ ] => tt
-    end
-  in
-  let cs :=
-    match goal with
-      | [ H : PropX.codeSpec _ _ |- _ ] => H
-    end
-  in
-  let ext' := 
-    match ext with
-      | _ => eval cbv delta [ ext ] in ext
-      | _ => ext
-    end
-  in
-  match stn_st_SF with
-    | tt => idtac (* nothing to symbolically evluate *)
-    | ((?stn, ?st), ?SF) =>
-      match find_reg st Rp with
-        | (?rp_v, ?rp_pf) =>
-          match find_reg st Sp with
-            | (?sp_v, ?sp_pf) =>
-              match find_reg st Rv with
-                | (?rv_v, ?rv_pf) =>
-(*TIME                  stop_timer "sym_eval:init" ; *)
-(*TIME                  start_timer "sym_eval:gather_instrs" ; *)
-                  let all_instrs := get_instrs st in
-                  let all_props := 
-                    ReifyExpr.collect_props ltac:(ILTacCommon.reflectable shouldReflect)
-                  in
-                  let pures := ReifyExpr.props_types all_props in
-                  let regs := constr:((rp_v, (sp_v, (rv_v, tt)))) in
-(*TIME                  stop_timer "sym_eval:gather_instrs" ; *)
-                  (** collect the raw types **)
-(*TIME                  start_timer "sym_eval:reify" ; *)
-                  let Ts := constr:(Reify.Tnil) in
-                  let Ts k := 
-                    match SF with
-                      | tt => k Ts
-                      | (?SF,_) => (** TODO: a little sketchy since it is in CPS **)
-                        SEP_REIFY.collectTypes_sexpr ltac:(isConst) SF Ts k 
-                    end
-                  in
-                    Ts ltac:(fun Ts => 
-                  collectAllTypes_instrs all_instrs Ts ltac:(fun Ts => 
-                  ReifyExpr.collectTypes_exprs ltac:(isConst) regs Ts ltac:(fun Ts => 
-                  ReifyExpr.collectTypes_exprs ltac:(isConst) pures Ts ltac:(fun Ts => 
-                  (** check for potential universe problems **)
-                  match Ts with
-                    | context [ PropX.PropX ] => 
-                      fail 1000 "found PropX in types list"
-                        "(this causes universe inconsistencies)" Ts
-                    | context [ PropX.spec ] => 
-                      fail 1000 "found PropX.spec in types list"
-                        "(this causes universe inconsistencies)" Ts
-                    | _ => idtac
-                  end;
-                  (** elaborate the types **)
-                  let types_ := reduce_repr ext tt (ILAlgoTypes.PACK.applyTypes (TacPackIL.ILAlgoTypes.Env ext) nil) in
-                  let types_ := ReifyExpr.extend_all_types Ts types_ in
-                  let typesV := fresh "types" in
-                  pose (typesV := types_);
-                  (** Check the types **)
-                  let pcT := constr:(Expr.tvType 0) in
-                  let stT := constr:(Expr.tvType 1) in
-                  (** build the variables **)
-                  let uvars := constr:(@nil (@sigT Expr.tvar (fun t : Expr.tvar => Expr.tvarD typesV t))) in
-                  let vars := uvars in
-                  (** build the base functions **)
-                  let funcs := reduce_repr ext tt (ILAlgoTypes.PACK.applyFuncs (TacPackIL.ILAlgoTypes.Env ext) typesV (repr (bedrock_funcs_r typesV) nil)) in
-                   (** build the base sfunctions **)
-(*                  let preds := constr:(@nil (@SEP.ssignature typesV pcT stT)) in *)
-                  let preds := reduce_repr ext tt (ILAlgoTypes.PACK.applyPreds (TacPackIL.ILAlgoTypes.Env ext) typesV nil) in
-                  (** reflect the expressions **)
-                  ReifyExpr.reify_exprs ltac:(isConst) pures typesV funcs uvars vars ltac:(fun uvars funcs pures =>
-                  let proofs := ReifyExpr.props_proof all_props in
-                  
-                  ReifyExpr.reify_expr ltac:(isConst) rp_v typesV funcs uvars vars ltac:(fun uvars funcs rp_v  => 
-                  ReifyExpr.reify_expr ltac:(isConst) sp_v typesV funcs uvars vars ltac:(fun uvars funcs sp_v =>  
-
-                  ReifyExpr.reify_expr ltac:(isConst) rv_v typesV funcs uvars vars ltac:(fun uvars funcs rv_v => 
-                    let finish H  :=
-(*TIME                      start_timer "sym_eval:cleanup" ; *)
-                      ((try exact H) ||
-                       (let rec destruct_exs H :=
-                         match type of H with
-                           | Logic.ex _ =>
-                             destruct H as [ ? H ] ; destruct_exs H
-                           | forall x : ?T, _ =>
-                             let n := fresh in
-                             evar (n : T); 
-                             let e := eval cbv delta [ n ] in n in 
-                             specialize (H e)                             
-                           | (_ /\ (_ /\ _)) /\ (_ /\ _) =>
-                             destruct H as [ [ ? [ ? ? ] ] [ ? ? ] ];
-                               repeat match goal with
-                                        | [ H' : _ /\ _ |- _ ] => destruct H'
-                                      end
-                           | False => destruct H
-                           | ?G =>
-                             fail 100000 "bad result goal" G
-                         end
-                        in let fresh Hcopy := fresh "Hcopy" in
-                          let T := type of H in
-                            assert (Hcopy : T) by apply H; clear H; destruct_exs Hcopy))
-(*TIME                    ;  stop_timer "sym_eval:cleanup" *)
-                    in
-                    build_path typesV all_instrs st uvars vars funcs ltac:(fun uvars funcs is fin_state is_pf => 
-                      match SF with
-                        | tt => 
-(*TIME                          stop_timer "sym_eval:reify" ; *)
-                          let funcsV := fresh "funcs" in
-                          pose (funcsV := funcs) ;
-                          let predsV := fresh "preds" in
-                          pose (predsV := preds) ;
-                          let uvarsV := fresh "uvars" in
-                          pose (uvarsV := uvars) ;
-(*                          let ExtC := constr:(@Algos_correct _ _ _ _ _ _ ext typesV funcsV predsV) in *)
-                          generalize (@SymILTac.ApplySymEval_slice_no_heap typesV funcsV predsV
-                            (@ILAlgoTypes.Algos ext typesV) (@ILAlgoTypes.Algos_correct ext typesV funcsV predsV)
-                            stn uvarsV)
-(*
-                          generalize (@SymILTac.stateD_proof_no_heap typesV funcsV predsV
-                            uvars st sp_v rv_v rp_v 
-                            sp_pf rv_pf rp_pf pures proofs cs stn) ;
-                          let H_stateD := fresh in
-                          intro H_stateD ;
-                          ((apply (@SymILTac.Apply_sym_eval typesV funcsV predsV
-                            (@ILAlgoTypes.Algos ext typesV) (@ILAlgoTypes.Algos_correct ext typesV funcsV predsV)
-                            stn uvars fin_state st is is_pf) in H_stateD)
-                          || fail 100000 "couldn't apply sym_eval_any! (non-SF case)"); 
-                          first [ simplifier typesV funcsV predsV H_stateD | fail 100000 "simplifier failed! (non-SF)" ] ;
-                          try clear typesV funcsV predsV ;
-                          first [ finish H_stateD (*; clear_instrs all_instrs*) | fail 100000 "finisher failed! (non-SF)" ] 
-*)
-                        | (?SF, ?H_interp) =>
-                          SEP_REIFY.reify_sexpr ltac:(isConst) SF typesV funcs pcT stT preds uvars vars 
-                          ltac:(fun uvars funcs preds SF =>
-(*TIME                            stop_timer "sym_eval:reify" ; *)
-(*TIME                            start_timer "sym_eval:pose" ; *)
-                            let funcsV := fresh "funcs" in
-                            pose (funcsV := funcs) ;
-                            let predsV := fresh "preds" in
-                            pose (predsV := preds) ;
-                            let uvarsV := fresh "uvars" in
-                            pose (uvarsV := uvars) ;
-                              idtac
-(*
-(*                            let ExtC := constr:(@Algos_correct ext typesV funcsV predsV) in *)
-(*TIME                            stop_timer "sym_eval:pose" ; *)
-(*TIME                            start_timer "sym_eval:apply_stateD_proof" ; *)
-                            apply (@SymILTac.stateD_proof typesV funcsV predsV
-                              uvars _ sp_v rv_v rp_v 
-                              sp_pf rv_pf rp_pf pures proofs SF _ _ (refl_equal _)) in H_interp ;
-(*TIME                            stop_timer "sym_eval:apply_stateD_proof" ; *)
-(*TIME                            start_timer "sym_eval:apply_sym_eval" ; *)
-                            ((apply (@SymILTac.Apply_sym_eval typesV funcsV predsV
-                              (@ILAlgoTypes.Algos ext typesV) (@ILAlgoTypes.Algos_correct ext typesV funcsV predsV)
-                              stn uvars fin_state st is is_pf) in H_interp) ||
-                             (idtac "couldn't apply sym_eval_any! (SF case)"; 
-                               first [ 
-                                 generalize (@SymILTac.Apply_sym_eval typesV funcsV predsV
-                                   (@ILAlgoTypes.Algos ext typesV) (@ILAlgoTypes.Algos_correct ext typesV funcsV predsV)
-                                   stn uvars fin_state st is is_pf) ; idtac "6" 
-                               | generalize (@SymILTac.Apply_sym_eval typesV funcsV predsV
-                                   (@ILAlgoTypes.Algos ext typesV) (@ILAlgoTypes.Algos_correct ext typesV funcsV predsV)
-                                   stn uvars fin_state st) ; idtac "5"  
-                               | generalize (@SymILTac.Apply_sym_eval typesV funcsV predsV
-                                   (@ILAlgoTypes.Algos ext typesV) (@ILAlgoTypes.Algos_correct ext typesV funcsV predsV)
-                                   stn uvars) ; idtac "4" 
-                               | generalize (@SymILTac.Apply_sym_eval typesV funcsV predsV
-                                   (@ILAlgoTypes.Algos ext typesV) (@ILAlgoTypes.Algos_correct ext typesV funcsV predsV)); idtac "3" 
-                               | generalize (@SymILTac.Apply_sym_eval typesV funcsV predsV
-                                   (@ILAlgoTypes.Algos ext typesV)) ; generalize (@ILAlgoTypes.Algos_correct ext typesV funcsV predsV) ; idtac "2" 
-                               | generalize (@SymILTac.Apply_sym_eval typesV funcsV predsV) ; idtac "1"  
-                               ])) ;
-(*TIME                             stop_timer "sym_eval:apply_sym_eval" ; *)
-(*TIME                             start_timer "sym_eval:simplify" ; *)
-                            first [ simplifier typesV funcsV predsV H_interp | fail 100000 "simplifier failed! (SF)" ] ;
-(*TIME                             stop_timer "sym_eval:simplify" ; *)
-(*TIME                             start_timer "sym_eval:clear" ; *)
-                            try clear typesV funcsV predsV ;
-(*TIME                             stop_timer "sym_eval:clear" ; *)
-                            first [ finish H_interp ; clear_instrs all_instrs | fail 100000 "finisher failed! (SF)" ]
-*) )
-                      end)))))  ))))
-              end
-          end
-      end
-  end.
-*)
